"Module invariance" adequacy thm + full verification of the stack example

theories/stack.v
@@ -2,7 +2,52 @@ From iris.proofmode Require Import tactics.
 From iris.algebra Require Import auth excl.
 From iris.base_logic.lib Require Import invariants.
 From intensional.heap_lang Require Import lifting proofmode notation.
+From intensional.heap_lang Require Import adequacy.
 Set Default Proof Using "Type".
+
+Definition create_spec `{!heapG Σ} P0 (Stack: list val → val → iProp Σ) (create: val) : iProp Σ :=
+  {{{ P0 }}}
+    create #()
+  {{{ s, RET s; Stack [] s }}}.
+
+Definition push_spec `{!heapG Σ} (Stack: list val → val → iProp Σ) (push: val) : iProp Σ :=
+  ∀ l s x,
+     {{{ Stack l s }}}
+       push s x
+     {{{ RET #(); Stack (x :: l) s }}}.
+
+Definition pop_spec `{!heapG Σ} (Stack: list val → val → iProp Σ) (pop: val) : iProp Σ :=
+  ∀ l s,
+   {{{ Stack l s }}}
+     pop s
+   {{{ v, RET v;
+     match l with
+     | [] => ⌜ v = #() ⌝ ∗ Stack [] s
+     | x :: l' => ⌜ v = x ⌝ ∗ Stack l' s
+     end }}}.
+
+Definition stacklib_spec `{!heapG Σ} (P0 : iProp Σ) (lib: val): iProp Σ :=
+  ∃ (Stack : list val → val → iProp Σ),
+    match lib with
+    | (create, push, pop)%V =>
+      create_spec P0 Stack create ∗ push_spec Stack push ∗ pop_spec Stack pop
+    | _ => False
+    end.
+
+Instance stacklib_persistent `{!heapG Σ} P0 lib : Persistent (stacklib_spec P0 lib).
+Proof.
+  apply bi.exist_persistent. intro.
+  repeat case_match; try typeclasses eauto.
+Qed.
+
+
+Module Impl.
+Section S.
+Context {Σ: gFunctors}.
+Context `{heapG Σ}.
+
+Definition create : val :=
+  λ: "u", ref (InjL #()).
 
 Definition push : val :=
   λ: "s" "x",
@@ -21,9 +66,6 @@ Definition pop : val :=
       "x"
     end.
 
-Section Stack_API.
-Context `{!heapG Σ}.
-
 Fixpoint list_val (l: list val) (v: val) : iProp Σ :=
   match l with
   | [] => ⌜ v = NONEV ⌝
@@ -36,8 +78,15 @@ Fixpoint list_val (l: list val) (v: val) : iProp Σ :=
 Definition stack_val (l: list val) (v: val) : iProp Σ :=
   ∃ (ℓ: loc) lv, ⌜ v = #ℓ ⌝ ∗ ℓ ↦ lv ∗ list_val l lv.
 
+Lemma create_correct :
+  {{{ True }}} create #() {{{ s, RET s; stack_val [] s }}}.
+Proof.
+  rewrite /create. iIntros (φ) "_ Hφ".
+  wp_pures. wp_alloc ℓ. iApply "Hφ".
+  rewrite /stack_val. iExists _, _. iFrame. eauto.
+Qed.
 
-Lemma push_spec s x l :
+Lemma push_correct s x l :
   {{{ stack_val l s }}}
     push s x
   {{{ RET #(); stack_val (x :: l) s }}}.
@@ -53,7 +102,7 @@ Proof.
   iSplit; eauto. cbn. iExists _, _. by iFrame.
 Qed.
 
-Lemma pop_spec s l :
+Lemma pop_correct s l :
   {{{ stack_val l s }}}
     pop s
   {{{ v, RET v;
@@ -76,16 +125,35 @@ Proof.
     unfold stack_val. iExists _, _. by iFrame. }
 Qed.
 
-End Stack_API.
+Lemma correct : ⊢ stacklib_spec True (create, push, pop).
+Proof.
+  iIntros "". unfold stacklib_spec.
+  iExists stack_val. repeat iSplit.
+  iIntros (?); iApply create_correct.
+  iIntros (? ? ? ?); iApply push_correct.
+  iIntros (? ? ?); iApply pop_correct.
+Qed.
+
+End S.
+End Impl.
 
 
-Definition good_trace (t: list event): Prop :=
+Section Trace.
+
+Print event. (* event = string * val *)
+
+Definition good_stack_trace (t: list event): Prop :=
   ∀ (i: nat) (v: val),
     t !! i = Some ("pop", v) → v ≠ #() →
     ∃ j, (j < i)%nat ∧ t !! j = Some ("push", v).
 
-Lemma good_trace_push t v :
-  good_trace t → good_trace (t ++ [("push", v)]).
+Lemma good_stack_trace_nil : good_stack_trace [].
+Proof.
+  intros i v Hti. rewrite lookup_nil in Hti; congruence.
+Qed.
+
+Lemma good_stack_trace_push t v :
+  good_stack_trace t → good_stack_trace (t ++ [("push", v)]).
 Proof.
   intros Ht i u [Hi|[_ Hi]]%lookup_app_Some Hv; cycle 1.
   { set X := (i - length t)%nat in Hi. destruct X.
@@ -107,9 +175,9 @@ Proof.
   { subst. right. split; eauto. rewrite Nat.sub_diag //=. }
 Qed.
 
-Lemma good_trace_pop_nil t :
-  good_trace t →
-  good_trace (t ++ [("pop", #())]).
+Lemma good_stack_trace_pop_nil t :
+  good_stack_trace t →
+  good_stack_trace (t ++ [("pop", #())]).
 Proof.
   intros Hgood i v Hti Hv.
   apply lookup_snoc_Some in Hti as [Hti | [_ ?]].
@@ -118,10 +186,10 @@ Proof.
   { congruence. }
 Qed.
 
-Lemma good_trace_pop t v i :
-  good_trace t →
+Lemma good_stack_trace_pop t v i :
+  good_stack_trace t →
   t !! i = Some ("push", v) →
-  good_trace (t ++ [("pop", v)]).
+  good_stack_trace (t ++ [("pop", v)]).
 Proof.
   intros Hgood Hti j v' Htj Hv'.
   apply lookup_snoc_Some in Htj as [Htj|[-> Hvv']].
@@ -135,36 +203,64 @@ Proof.
     - rewrite lookup_app_l //. }
 Qed.
 
-Section Wrapped_Stack_API.
-Context `{!heapG Σ}.
+End Trace.
+
+
+Module Wrap.
+Section S.
+Context {Σ: gFunctors}.
+Context `{heapG Σ}.
 Context (N: namespace).
 
-Definition stack_val' (l: list val) (v: val) : iProp Σ :=
-  stack_val l v ∗ trace_inv N good_trace ∗
-  ∃ t, trace_is t ∗ ⌜good_trace t⌝ ∗
+Context (stack_impl: list val → val → iProp Σ).
+Context (push_impl pop_impl create_impl : val).
+
+Definition push : val :=
+  λ: "s" "x", push_impl "s" "x" ;; Emit "push" "x".
+
+Definition pop : val :=
+  λ: "s", let: "r" := pop_impl "s" in Emit "pop" "r" ;; "r".
+
+Definition create : val :=
+  create_impl.
+
+Definition stack_val (l: list val) (v: val) : iProp Σ :=
+  stack_impl l v ∗ trace_inv N good_stack_trace ∗
+  ∃ t, trace_is t ∗ ⌜good_stack_trace t⌝ ∗
   ⌜ Forall (λ x, ∃ i, t !! i = Some ("push", x)) l ⌝.
 
-Definition push' : val :=
-  λ: "s" "x", push "s" "x" ;; Emit "push" "x".
-
-Definition pop' : val :=
-  λ: "s", let: "r" := pop "s" in Emit "pop" "r" ;; "r".
-
-Lemma push'_spec s x l :
-  {{{ stack_val' l s }}}
-    push' s x
-  {{{ RET #(); stack_val' (x :: l) s }}}.
+Lemma create_correct P0 :
+  create_spec P0 stack_impl create_impl -∗
+  {{{ P0 ∗ trace_is [] ∗ trace_inv N good_stack_trace }}}
+    create #()
+  {{{ s, RET s; stack_val [] s }}}.
 Proof.
-  iIntros (φ) "Hs Hφ". unfold push'.
+  iIntros "#create_impl_spec". iModIntro.
+  iIntros (φ) "(H0 & Htr & HI) Hφ". unfold create.
+  iApply ("create_impl_spec" with "[$]").
+  iIntros "!>" (?) "?". iApply "Hφ". rewrite /stack_val.
+  iFrame. iExists []. iFrame. iPureIntro; split.
+  by apply good_stack_trace_nil.
+  by apply Forall_nil.
+Qed.
+
+Lemma push_correct s x l :
+  push_spec stack_impl push_impl -∗
+  {{{ stack_val l s }}}
+    push s x
+  {{{ RET #(); stack_val (x :: l) s }}}.
+Proof.
+  iIntros "#push_impl_spec". iModIntro.
+  iIntros (φ) "Hs Hφ". unfold push.
   iDestruct "Hs" as "(Hs & #HI & Htr)". iDestruct "Htr" as (t) "(Ht & Hgood & HF)".
   iDestruct "Hgood" as %Hgood. iDestruct "HF" as %HF.
-  wp_pures. wp_bind (push _ _).
-  iApply (push_spec with "Hs"). iIntros "!> Hs".
+  wp_pures. wp_bind (push_impl _ _).
+  iApply ("push_impl_spec" with "Hs"). iIntros "!> Hs".
   wp_pures.
-  eapply good_trace_push in Hgood.
+  eapply good_stack_trace_push in Hgood.
   iApply (wp_emit with "[$Ht $HI]"); eauto.
   iIntros "!> Ht". iApply "Hφ".
-  rewrite /stack_val'; iFrame "HI∗".
+  rewrite /stack_val; iFrame "HI∗".
   iExists _; iFrame. iPureIntro; split; eauto.
   rewrite Forall_cons. split.
   { exists (length t). by apply list_lookup_middle. }
@@ -172,34 +268,36 @@ Proof.
     intros v [i Hti]. exists i. by apply lookup_app_l_Some. }
 Qed.
 
-Lemma pop'_spec s l :
-  {{{ stack_val' l s }}}
-    pop' s
+Lemma pop_correct s l :
+  pop_spec stack_impl pop_impl -∗
+  {{{ stack_val l s }}}
+    pop s
   {{{ v, RET v;
       match l with
-      | [] => ⌜ v = #() ⌝ ∗ stack_val' [] s
-      | x :: l' => ⌜ v = x ⌝ ∗ stack_val' l' s
+      | [] => ⌜ v = #() ⌝ ∗ stack_val [] s
+      | x :: l' => ⌜ v = x ⌝ ∗ stack_val l' s
       end }}}.
 Proof.
-  iIntros (φ) "Hs Hφ". unfold pop'.
+  iIntros "#pop_impl_spec". iModIntro.
+  iIntros (φ) "Hs Hφ". unfold pop.
   iDestruct "Hs" as "(Hs & #HI & Htr)". iDestruct "Htr" as (t) "(Ht & Hgood & HF)".
   iDestruct "Hgood" as %Hgood. iDestruct "HF" as %HF.
-  wp_pures. wp_bind (pop _).
-  iApply (pop_spec with "Hs"). iIntros "!>" (v) "Hs".
+  wp_pures. wp_bind (pop_impl _).
+  iApply ("pop_impl_spec" with "Hs"). iIntros "!>" (v) "Hs".
   wp_pures. wp_bind (Emit _ _).
   destruct l as [|x l'].
   { iDestruct "Hs" as "(-> & Hs)".
-    apply good_trace_pop_nil in Hgood.
+    apply good_stack_trace_pop_nil in Hgood.
     iApply (wp_emit with "[$Ht $HI]"); eauto.
     iIntros "!> Ht". wp_pures. iApply "Hφ". iSplitR; first done.
-    rewrite /stack_val'; iFrame "HI∗".
+    rewrite /stack_val; iFrame "HI∗".
     iExists _. iFrame. iPureIntro; split; eauto. }
   { iDestruct "Hs" as "(-> & Hs)".
     apply Forall_cons in HF as [[i Hti] HF].
-    eapply good_trace_pop in Hgood; eauto.
+    eapply good_stack_trace_pop in Hgood; eauto.
     iApply (wp_emit with "[$Ht $HI]"); eauto.
     iIntros "!> Ht". wp_pures. iApply "Hφ". iSplitR; first done.
-    rewrite /stack_val'; iFrame "HI∗".
+    rewrite /stack_val; iFrame "HI∗".
     iExists _. iFrame. iPureIntro; split; eauto.
     eapply Forall_impl; [ apply HF |]. cbn.
     intros v [j Htj].
@@ -209,4 +307,47 @@ Proof.
     { exists j. rewrite lookup_app_l //. apply lookup_lt_is_Some_1; eauto. } }
 Qed.
 
-End Wrapped_Stack_API.
+End S.
+
+Definition lib (lib_impl: val): val :=
+  match lib_impl with
+  | (create_impl, push_impl, pop_impl)%V =>
+    (create create_impl, push push_impl, pop pop_impl)
+  | _ => #()
+  end.
+
+Lemma correct `{!heapG Σ} N P0 (lib_impl: val) :
+  stacklib_spec P0 lib_impl -∗
+  stacklib_spec (P0 ∗ trace_is [] ∗ trace_inv N good_stack_trace) (lib lib_impl).
+Proof.
+  iIntros "#S". iDestruct "S" as (stack_val_impl) "S".
+  repeat case_match; eauto. iDestruct "S" as "(Hcreate & Hpush & Hpop)".
+  subst. unfold stacklib_spec.
+  iExists (stack_val N stack_val_impl). repeat iSplit.
+  iApply create_correct; eauto.
+  iIntros (? ? ?); iApply push_correct; eauto.
+  iIntros (? ?); iApply pop_correct; eauto.
+Qed.
+
+End Wrap.
+
+
+Definition stacklibN := nroot .@ "stacklib".
+Definition empty_state : state := Build_state ∅ [] ∅.
+
+Lemma wrap_stacklib_correct {Σ} `{heapPreG Σ} (e: val → expr) (lib: val):
+  (⊢ ∀ `{heapG Σ}, stacklib_spec True lib) →
+  (⊢ ∀ `{heapG Σ} P lib, stacklib_spec P lib -∗ {{{ P }}} e lib {{{ v, RET v; True }}}) →
+  ∀ σ' e',
+    rtc erased_step ([(#();; e (Wrap.lib lib))%E], empty_state) (e', σ') →
+    good_stack_trace (trace σ').
+Proof.
+  intros Hlib Hctx σ' e' Hsteps.
+  eapply (@module_invariance Σ _ stacklibN (@stacklib_spec Σ) True e #() (Wrap.lib lib)
+                            good_stack_trace empty_state).
+  { cbn. apply good_stack_trace_nil. }
+  { iIntros (? ? ?) "?". by iApply Hctx. }
+  { iIntros (? _) "!>". iApply wp_value; eauto. }
+  { iIntros (?). iApply Wrap.correct. iApply Hlib. }
+  eauto.
+Qed.
