theories/heap_lang/adequacy.v
@@ -53,3 +53,39 @@ Proof.
   iInv "HI" as ">Ht'" "_". iDestruct "Ht'" as (t') "(Ht' & %)".
   iDestruct (trace_auth_half_frag_agree with "Hta Ht'") as %->. iModIntro. eauto.
 Qed.
+
+Require Import iris.program_logic.hoare.
+
+Lemma module_invariance {Σ} `{heapPreG Σ} (N: namespace)
+  (Φ: ∀ `{heapG Σ}, iProp Σ → val → iProp Σ)  (* Module specification *)
+  (P0: iProp Σ) (* Initial resources required by the module *)
+  (e: val → expr) (* Context program, parameterized by the module *)
+  (e_init: expr) (* Initialization code, used to allocate resources for P0 *)
+  (imimpl: val) (* Implementation of the module (instrumented) *)
+  (good_trace: list event → Prop) (* Trace property *)
+  (σ: state) (* Initial state *)
+:
+  (* The initial trace must satisfy the property *)
+  good_trace (trace σ) →
+  (* The context must be safe, given a module satisfying the specification Φ *)
+  (⊢ ∀ `{heapG Σ} P m, Φ P m -∗ {{{ P }}} e m {{{ v, RET v; True }}}) →
+  (* The initialization code must provide P0 *)
+  (⊢ ∀ `{heapG Σ}, {{ True }} e_init {{ _, P0 }}) →
+  (* The implementation provided for the module (iops) must satisfy the specification Φ.
+     On top of P0 it is given SL resources for the trace. *)
+  (⊢ ∀ `{heapG Σ}, Φ (P0 ∗ trace_is (trace σ) ∗ trace_inv N good_trace)%I imimpl) →
+  (* Then the trace remains good at every step *)
+  ∀ σ' e',
+    rtc erased_step ([(e_init;; e imimpl)%E], σ) (e', σ') →
+    good_trace (trace σ').
+Proof.
+  intros Htrσ Hctx Hinit Himpl σ' e' Hsteps.
+  eapply heap_invariance. done. by apply Htrσ. 2: eapply Hsteps.
+  iIntros (?) "HI Htr". wp_bind e_init.
+  iApply wp_wand. by iApply Hinit.
+  iIntros (v) "H0". wp_pures.
+  iApply (Hctx with "[] [H0 Htr HI]").
+  - iApply Himpl.
+  - iFrame.
+  - eauto.
+Qed.
